Port LLVMExceptions.v and Denotations.v (modulo mrec).

src/rocq/Handlers/LLVMExceptions.v
@@ -8,18 +8,23 @@ From ExtLib Require Import
   Structures.Monads
   EitherMonad.
 
-From ITree Require Import
-     ITree
-     Eq.Eqit
-     InterpFacts.
-
 From Vellvm Require Import
      Utils.Util
      Utils.Error
      Utils.Tactics
      Utils.InterpEither
+     Utils.CTreeUtils
+     Utils.Monads
      Semantics.LLVMEvents
      Semantics.Memory.Sizeof.
+
+From CTree Require Import
+  CTree
+  Fold
+  FoldCTree
+  FoldStateT
+  Eq
+  SBisim.
 
 Require Import Ceres.Ceres.
 
@@ -30,6 +35,8 @@ Import MonadNotation.
 Import ITree.Basics.Basics.Monads.
 Open Scope string_scope.
 Open Scope monad.
+
+Import CategoryOps.
 (* end hide *)
 
 
@@ -47,30 +54,30 @@ Section Exceptions.
       end.
 
   Section LLVMExcHandler.
-    Variable (E F G : Type -> Type).
+    Variable (E F G BR : Type -> Type).
     Context `{FAIL: FailureE -< G}.
     Notation Effin := (E +' F +' LLVMExcE EXC +' G).
     Notation Effout := (E +' F +' LLVMExcE EXC +' G).
 
-    Definition E_trigger : forall R, E R -> eitherT EXC (itree Effout) R :=
+    Definition E_trigger : forall R, E R -> eitherT EXC (ctree Effout BR) R :=
       fun R e => mkEitherT (r <- trigger e ;; ret (inr r)).
 
-    Definition F_trigger : forall R, F R -> eitherT EXC (itree Effout) R :=
+    Definition F_trigger : forall R, F R -> eitherT EXC (ctree Effout BR) R :=
       fun R e => mkEitherT (r <- trigger e ;; ret (inr r)).
 
-    Definition G_trigger : forall R, G R -> eitherT EXC (itree Effout) R :=
+    Definition G_trigger : forall R, G R -> eitherT EXC (ctree Effout BR) R :=
       fun R e => mkEitherT (r <- trigger e ;; ret (inr r)).
 
-    Definition catch_llvm_exc_h : IFun Effin (fun R : Type => eitherT EXC (itree Effout) R)
-      := (case_ E_trigger (case_ F_trigger (case_ (@handle_LLVMExcE (itree Effout) _) G_trigger))).
+    Definition catch_llvm_exc_h : IFun Effin (fun R : Type => eitherT EXC (ctree Effout BR) R)
+      := (case_ E_trigger (case_ F_trigger (case_ (@handle_LLVMExcE (ctree Effout BR) _) G_trigger))).
 
-    Definition catch_llvm_exc : itree Effin ~> eitherT EXC (itree Effout)
+    Definition catch_llvm_exc : ctree Effin BR ~> eitherT EXC (ctree Effout BR)
       := interp_either catch_llvm_exc_h.
 
     Section Structural_Lemmas.
       Lemma catch_llvm_exc_bind :
-        forall (R S : Type) (t : itree Effin R) (k : R -> itree Effin S),
-          Monad.eq1 (catch_llvm_exc (ITree.bind t k))
+        forall (R S : Type) (t : ctree Effin BR R) (k : R -> ctree Effin BR S),
+          Monad.eq1 (catch_llvm_exc (CTree.bind t k))
             (r <- catch_llvm_exc t;; catch_llvm_exc (k r)).
       Proof using E EXC F G FAIL.
         intros.
@@ -81,25 +88,25 @@ Section Exceptions.
 
       Lemma catch_llvm_exc_ret :
         forall (R : Type) (x: R),
-          Monad.eq1 (catch_llvm_exc (Ret x: itree Effin R)) (ret x).
+          Monad.eq1 (catch_llvm_exc (Ret x: ctree Effin BR R)) (ret x).
       Proof using.
         intros.
         unfold catch_llvm_exc.
         apply interp_either_ret.
       Qed.
 
-      Lemma catch_llvm_exc_Tau :
-        forall {R} (t: itree Effin R),
-          Monad.eq1 (catch_llvm_exc (Tau t)) (catch_llvm_exc t).
+      Lemma catch_llvm_exc_Guard :
+        forall {R} (t: ctree Effin BR R),
+          Monad.eq1 (catch_llvm_exc (Guard t)) (catch_llvm_exc t).
       Proof using.
         intros.
         unfold catch_llvm_exc.
-        apply interp_either_tau.
+        apply interp_either_guard.
       Qed.
 
       Lemma catch_llvm_exc_vis:
-        forall S X (kk : X -> itree Effout S) (e : Effin X),
-          @Monad.eq1 (eitherT EXC (itree Effout)) _ _ (@catch_llvm_exc S (Vis e kk)) (@bind (eitherT EXC (itree Effout)) _ _ _ (@catch_llvm_exc_h X e) (fun sx => @catch_llvm_exc S (kk sx))).
+        forall S X (kk : X -> ctree Effout BR S) (e : Effin X),
+          @Monad.eq1 (eitherT EXC (ctree Effout BR)) _ _ (@catch_llvm_exc S (Vis e kk)) (@bind (eitherT EXC (ctree Effout BR)) _ _ _ (@catch_llvm_exc_h X e) (fun sx => @catch_llvm_exc S (kk sx))).
       Proof using.
         intros.
         unfold catch_llvm_exc.
@@ -109,7 +116,7 @@ Section Exceptions.
 
       Lemma catch_llvm_exc_trigger:
         forall X (e : Effin X),
-          Monad.eq1 (catch_llvm_exc (ITree.trigger e)) (catch_llvm_exc_h e).
+          @Monad.eq1 _ EqM_eitherT _  (catch_llvm_exc (CTree.trigger e)) (catch_llvm_exc_h e).
       Proof using.
         intros.
         unfold catch_llvm_exc.
@@ -117,33 +124,33 @@ Section Exceptions.
         reflexivity.
       Qed.
 
-      Lemma catch_llvm_exc_bind_trigger_eqit:
-        forall X R
-          (kk : X -> itree Effin R)
-          (e : Effin X),
-          eq_either_itree (catch_llvm_exc (ITree.bind (trigger e) kk)) (@bind (eitherT EXC (itree Effout)) _ _ _ (catch_llvm_exc_h e) (fun x => catch_llvm_exc (Tau (kk x)))).
-      Proof using.
-        intros.
-        unfold catch_llvm_exc.
-        rewrite bind_trigger.
-        setoid_rewrite interp_either_vis'.
-        reflexivity.
-      Qed.
+      (* Lemma catch_llvm_exc_bind_trigger_eqit: *)
+      (*   forall X R *)
+      (*     (kk : X -> ctree Effin BR R) *)
+      (*     (e : Effin X), *)
+      (*     eq_either_itree (catch_llvm_exc (CTree.bind (trigger e) kk)) (@bind (eitherT EXC (ctree Effout BR)) _ _ _ (catch_llvm_exc_h e) (fun x => catch_llvm_exc (Guard (kk x)))). *)
+      (* Proof using. *)
+      (*   intros. *)
+      (*   unfold catch_llvm_exc. *)
+      (*   rewrite bind_trigger. *)
+      (*   setoid_rewrite interp_either_vis'. *)
+      (*   reflexivity. *)
+      (* Qed. *)
 
-      Lemma catch_llvm_exc_bind_trigger:
-        forall X R
-          (kk : X -> itree Effin R)
-          (e : Effin X),
-          Monad.eq1 (catch_llvm_exc (ITree.bind (trigger e) kk)) (@bind (eitherT EXC (itree Effout)) _ _ _ (catch_llvm_exc_h e) (fun x => catch_llvm_exc (kk x))).
-      Proof using.
-        intros.
-        rewrite catch_llvm_exc_bind_trigger_eqit.
-        setoid_rewrite catch_llvm_exc_Tau.
-        reflexivity.
-      Qed.
+      (* Lemma catch_llvm_exc_bind_trigger: *)
+      (*   forall X R *)
+      (*     (kk : X -> ctree Effin BR R) *)
+      (*     (e : Effin X), *)
+      (*     Monad.eq1 (catch_llvm_exc (CTree.bind (trigger e) kk)) (@bind (eitherT EXC (ctree Effout BR)) _ _ _ (catch_llvm_exc_h e) (fun x => catch_llvm_exc (kk x))). *)
+      (* Proof using. *)
+      (*   intros. *)
+      (*   rewrite catch_llvm_exc_bind_trigger_eqit. *)
+      (*   setoid_rewrite catch_llvm_exc_Guard. *)
+      (*   reflexivity. *)
+      (* Qed. *)
 
       #[global] Instance eutt_catch_llvm_exc {R} :
-        Proper (eutt eq ==> Monad.eq1) (@catch_llvm_exc R).
+        Proper (sbisim eq  ==> Monad.eq1) (@catch_llvm_exc R).
       Proof using.
         repeat intro.
         unfold catch_llvm_exc.
